Splinter/Allocation.i.dfy
@@ -8,16 +8,17 @@ module AllocationMod {
   function DiskSizeInAU() : (s:nat)
     ensures 1<=s
 
-  function AUSizeInBlocks() : (s:nat)
-    ensures 2<=s
+  function AUSizeInCUs() : (s:nat)
+    ensures 2<=s  // TODO(jonh): explain why
 
   predicate ValidCU(cu: CU) {
     && 0 <= cu.au < DiskSizeInAU()
-    && 0 <= cu.offset < AUSizeInBlocks()
+    && 0 <= cu.offset < AUSizeInCUs()
   }
 
   type DiskView = map<CU, UninterpretedDiskPage>
 
+  // TODO(jonh): robj points out we should have a ValidView first, then fullness later.
   predicate FullView(dv: DiskView) {
     forall cu :: cu in dv.Keys <==> ValidCU(cu)
   }
@@ -28,6 +29,7 @@ module AllocationMod {
     || (cu in dv0 && cu in dv1 && dv0[cu]==dv1[cu])
   }
 
+  // TODO: this should probably be defined over CUs.
   predicate DiskViewsEquivalentForSet(dv0: DiskView, dv1: DiskView, aus: seq<AU>)
   {
     forall cu:CU :: cu.au in aus ==> EqualAt(dv0, dv1, cu)
