Splinter/Program.i.dfy
@@ -1,0 +1,208 @@
+include "Journal.i.dfy"
+include "Betree.i.dfy"
+
+// The "Program" is the complete model of the program state, with all of the components
+// (Journal, Betree, Cache).
+// It has an interface to a disk, but can't actually see inside the disk (that's for the IOSystem).
+
+module ProgramMachineMod {
+  datatype Superblock = Superblock(
+    serial: nat,
+    journal: JournalMod.Superblock,
+    betree: BetreeMod.Superblock)
+
+  datatype Variables = Variables(
+    stableSuperblock: Superblock,
+    journal: JournalMachine.Variables,
+    betree: CachedBetreeMachine.Variables,
+    inFlightSuperblock: Option<Superblock>
+    )
+  {
+    predicate WF() {
+      true
+    }
+  }
+
+  predicate Init(s: Variables)
+  {
+  }
+
+  predicate Recover(s: Variables, s': Variables)
+  {
+  }
+
+  predicate Query(s: Variables, s': Variables, k: Key, v: Value)
+  {
+    && s.WF()
+    && s'.journal == s.journal
+    && CachedBetreeMachine.Query(s, s', k, v)
+  }
+
+  predicate Put(s: Variables, s': Variables, k: Key, v: Value)
+  {
+    && s.WF()
+    && JournalMachine.Record(s, s', JournalMachine.Put(k, v))
+    && CachedBetreeMachine.Put(s, s', k, v)
+  }
+
+  predicate BetreeNoop(s: Variables, s': Variables)
+  {
+    && s.WF()
+    && s'.journal == s.journal
+    && CachedBetreeMachine.Noop(s, s')
+  }
+
+  predicate AsyncFlush(s: Variables, s': Variables)
+  {
+    && s.WF()
+    && JournalMachine.AsyncFlush(s, s')
+    && CachedBetreeMachine.Noop(s, s')
+  }
+
+  predicate ReqSync(s: Variables, s': Variables, syncReqId: SyncReqId)
+  {
+    && s.WF()
+    && JournalMachine.ReqSync(s, s', syncReqId)
+    && CachedBetreeMachine.Noop(s, s')
+  }
+ 
+  predicate CompleteSync(s: Variables, s': Variables, syncReqId: SyncReqId)
+  {
+    && s.WF()
+    && JournalMachine.CompleteSync(s, s', syncReqId)
+    && CachedBetreeMachine.Noop(s, s')
+  }
+
+  // At some lower layer, where we duplicate the superblock to protect against disk sector
+  // corruption, the Commit sequence looks like this:
+  //   write sb0
+  //   complete: ensure sb0 has hit the disk successfully before writing sb1, which might tear
+  //   write sb1
+  //   complete: Tell subsystems the commit is done. Can't acknowledge a sync dependent on this sb
+  //     until sb1 commits, lest sb0 get lost before sb1 is successfully written and the "synced"
+  //     data gets lost
+  // At this layer, we abbreviate that to "write sb" and "write sb complete".
+  predicate CommitStart(s: Variables, s': Variables, seqBoundary: nat)
+  {
+    && s.inFlightSuperblock.None?
+    && var sb := s'.inFlightSuperblock;
+    && Journal.CommitStart(s.journal, s'.journal, sb.journal, seqBoundary)
+    && Betree.CommitStart(s.betree, s'.betree, sb.betree, seqBoundary)
+    && sb.serial == s.stableSuperblock.serial + 1
+    && Disk.IssueWrite(s, s', SUPERBLOCK_ADDRESS(), sb) // TODO this stuff comes in as a binding param
+  }
+
+  predicate CommitComplete(s: Variables, s': Variables)
+  {
+    && Disk.CompleteWrite(s, s', ?)   // how to match the write req?
+    && s.inFlightSuperblock.Some?
+    && var sb := s.inFlightSuperblock.value;
+    && s'.stableSuperblock == sb
+    && Journal.CommitComplete(s.journal, s'.journal, sb.journal)
+    && Betree.CommitComplete(s.betree, s'.betree, sb.betree)
+    && s'.inFlightSuperblock.None?
+  }
+
+  predicate Next(s: Variables, s': Variables) {
+    exists step ::
+      && NextStep(s, s', step)
+      && AllocationTablesDisjoint(s'.journal.allocation, s'.betree.allocation)
+  }
+}
+
+module ProgramInterpMod {
+  import opened Options
+  import opened MessageMod
+  import opened InterpMod
+  import opened AllocationMod
+  import opened MsgSeqMod
+  import AllocationTableMod
+  import JournalMod
+  import BetreeMod
+
+  function parseSuperblock(b: UninterpretedDiskPage) : Option<Superblock>
+
+  function ISuperblock(dv: DiskView) : Option<Superblock>
+  {
+    var bcu0 := CU(0, 0);
+    var bcu1 := CU(0, 1);
+    if bcu0 in dv && bcu1 in dv
+    then
+      var sb0 := parseSuperblock(dv[bcu0]);
+      var sb1 := parseSuperblock(dv[bcu1]);
+      if sb0.Some? && sb1.Some? && sb0.value.serial == sb1.value.serial
+      then
+        sb0
+      else
+        None  // Stop! Recovery should ... copy the newer one?
+          // well I think I() of that should be the newer one, but we should just
+          // not be allowed to write anything until we've got them back in sync.
+    else
+      None  // silly expression: DV has holes in it
+  }
+
+  function ISuperblockReads(dv: DiskView) : set<AU>
+  {
+    {0}
+  }
+ 
+  // IM == Interpret as InterpMod
+  // Oh man we're gonna have a family of IReads predicates that capture the
+  // heapiness of DiskView, aren't we?
+  function IM(dv: DiskView) : (i:Interp)
+    ensures i.WF()
+  {
+    var sb := ISuperblock(dv);
+    if sb.Some?
+    then
+      Concat(BetreeMod.IM(dv, sb.value.betree), JournalMod.IM(dv, sb.value.journal))
+    else
+      InterpMod.Empty()
+  }
+
+  function IMReads(dv: DiskView) : seq<AU> {
+      []
+      /*
+    var sb := ISuperblock(dv);
+    if sb.Some?
+    then
+      JournalMod.IReads(dv, sb.value.journal) + BetreeMod.IReads(dv, sb.value.betree)
+    else
+      set{}
+      */
+  }
+
+  function IReads(dv: DiskView) : seq<AU> {
+    IMReads(dv)
+  }
+
+  lemma Framing(dv0: DiskView, dv1: DiskView)
+    requires DiskViewsEquivalentForSet(dv0, dv1, IReads(dv0))
+    ensures IM(dv0) == IM(dv1)
+  {
+    //assert forall k :: k !in I(dv0);
+    //assert forall k :: IM(dv0).mi[k] == IM(dv1).mi[k];
+  }
+}
+
+/*
+Okay, so the magic is going to be that
+- most of the time when we change a block in RAM we'll prove that it's
+  not in use in any other view
+  - that'll depend on an invariant between the allocation table
+    and the IReads functions
+  - And we'll need a proof that, if IReads doesn't change, I doesn't
+    change, of course.
+- when we write a non-superblock back to disk, we inherit that no-change
+  property; the persistent view doesn't change because the thing
+  we wrote back was dirty and hence outside of the IReads of the
+  persistent view.
+- when we update the superblock, we're creating a frozen view.
+- when we write a superblock back, it's easy again, because the persistent
+  view just vanishes, replaced by the frozen view.
+  The vanishing old persistent view implicitly creates some free nodes,
+  which can be detected because the available nodes are computed at
+  runtime by reading the active AllocationTables, and one just became
+  empty.
+  (that is, the union of allocationTables will cover the IReads sets.)
+*/
